Support unsat-core and counter-examples. (#196)
* Provide initial support for unsat-core and counter-examples.

* Improve model support and disable it by default.

Smt/Tactic/Smt.lean
@@ -6,6 +6,7 @@ Authors: Abdalrhman Mohamed
 -/
 
 import Lean
+import Lean.Meta.Tactic.TryThis
 
 import Smt.Dsl.Sexp
 import Smt.Reconstruct
@@ -13,7 +14,6 @@ import Smt.Reconstruct.Prop.Lemmas
 import Smt.Translate.Query
 import Smt.Preprocess
 import Smt.Util
-import Smt.Auto
 
 namespace Smt
 
@@ -28,40 +28,33 @@ structure Config where
   /-- Whether to enable native components for proof reconstruction. Speeds up normalization and
       reduction proof steps. However, it adds the Lean compiler to the trusted code base. -/
   native : Bool := false
-  /-- Whether to preprocess the query before sending it to the SMT solver. -/
-  preprocess : Bool := true
-  /-- Whether to monomorphize the Lean goal before invoking the SMT solver. -/
+  /-- Whether to monomorphize the Lean goal before sending it to the SMT solver. -/
   mono : Bool := false
+  /-- Whether to eliminate `↔` in the Lean goal before sending it to the SMT solver. -/
+  elimIff : Bool := true
   /-- Whether to trust the result of the SMT solver. Closes the current goal with a `sorry` if the
       SMT solver returns `unsat`. **Warning**: use with caution, as this may lead to unsoundness.
       Additionally adds the translation from Lean to SMT to the trusted code base, which is not
       always sound. -/
   trust : Bool := false
+  /-- Whether to show a potential counter-example when the SMT solver returns `sat`. -/
+  model : Bool := false
   /-- Just show the SMT query without invoking a solver. Useful for debugging. -/
   showQuery : Bool := false
 deriving Inhabited, Repr
 
-/-- Return all propositions in the local context. -/
-def getPropHyps : MetaM (Array FVarId) := do
-  let mut result := #[]
-  for localDecl in (← getLCtx) do
-    unless localDecl.isImplementationDetail do
-      if ← pure !(isNonEmpty localDecl.type) <&&> Meta.isProp localDecl.type then
-        result := result.push localDecl.fvarId
-  return result
-where
-  isNonEmpty (e : Expr) : Bool :=
-  match_expr e with
-  | Nonempty _ => true
-  | _ => false
+inductive Result where
+  | sat (model : Option (Array (Expr × Expr)))
+  | unsat (mvs : List MVarId) (usedHints : Array Expr)
+  | unknown (reason : String)
 
-def genUniqueFVarNames : MetaM (Std.HashMap FVarId String × Std.HashMap String FVarId) := do
+def genUniqueFVarNames : MetaM (Std.HashMap FVarId String × Std.HashMap String Expr) := do
   let lCtx ← getLCtx
   let st : NameSanitizerState := { options := {}}
   let (lCtx, _) := (lCtx.sanitizeNames st).run
   return lCtx.getFVarIds.foldl (init := ({}, {})) fun (m₁, m₂) fvarId =>
     let m₁ := m₁.insert fvarId (lCtx.getRoundtrippingUserName? fvarId).get!.toString
-    let m₂ := m₂.insert (lCtx.getRoundtrippingUserName? fvarId).get!.toString fvarId
+    let m₂ := m₂.insert (lCtx.getRoundtrippingUserName? fvarId).get!.toString (.fvar fvarId)
     (m₁, m₂)
 
 def prepareSmtQuery (hs : List Expr) (goalType : Expr) (fvNames : Std.HashMap FVarId String) : MetaM (List Command) := do
@@ -69,46 +62,23 @@ def prepareSmtQuery (hs : List Expr) (goalType : Expr) (fvNames : Std.HashMap FV
   Lean.Meta.withLocalDeclD goalId.name (mkNot goalType) fun g =>
   Query.generateQuery g hs fvNames
 
-def withProcessedHints (mv : MVarId) (hints : Auto.InputHints') (k : MVarId → List Expr → MetaM α) : MetaM α := do
-  let mut hs := hints.lemmas.map (·.proof)
-  if hints.lctxhyps then
-    hs := hs ++ (← getPropHyps).toList.map Expr.fvar
-  go mv hs.toList [] k
-where
-  go (mv : MVarId) (hs : List Expr) (fvs : List Expr) (k : MVarId → List Expr → MetaM α): MetaM α := do
-    match hs with
-    | [] => k mv fvs
-    | h :: hs =>
-      if h.isFVar || h.isConst then
-        go mv hs (h :: fvs) k
-      else
-        let mv ← mv.assert (← mkFreshId) (← Meta.inferType h) h
-        let ⟨fv, mv⟩ ← mv.intro1
-        go mv hs (.fvar fv :: fvs) k
-
-def withMono (mv : MVarId) (hs : Auto.InputHints') (k : MVarId → List Expr → MetaM α) : MetaM α := do
-  let (mv, _) ← Auto.mono' `smt mv hs #[] #[]
-  let hs ← mv.withContext (return (← Smt.getPropHyps).toList.map Expr.fvar)
-  trace[smt] "goal: {mv}"
-  k mv hs
-
-def smt (cfg : Config) (mv : MVarId) (hs : Auto.InputHints') : MetaM (List MVarId) := mv.withContext do
+def smt (cfg : Config) (mv : MVarId) (hs : Array Expr) : MetaM Result := mv.withContext do
   -- 0. Create a duplicate goal to preserve the original goal.
   let mv₁ := (← Meta.mkFreshExprMVar (← mv.getType)).mvarId!
   -- 1. Process the hints passed to the tactic.
-  (if cfg.mono then withMono else withProcessedHints) mv₁ hs fun mv₂ hs => mv₂.withContext do
+  let ⟨map₁, hs₁, mv₂⟩ ← (if cfg.mono then Preprocess.mono else Preprocess.pushHintsToCtx) mv₁ hs
   -- 2. Preprocess the hypotheses and goal.
-  let (hs, mv₂) ← if cfg.preprocess then Preprocess.elimIff mv₂ hs else pure (hs, mv₂)
+  let ⟨map₂, hs₂, mv₂⟩ ← if cfg.elimIff then Preprocess.elimIff mv₂ hs₁ else pure ⟨map₁, hs₁, mv₂⟩
   mv₂.withContext do
   let goalType : Q(Prop) ← mv₂.getType
   -- 3. Generate the SMT query.
   let (fvNames₁, fvNames₂) ← genUniqueFVarNames
-  let cmds ← prepareSmtQuery hs (← mv₂.getType) fvNames₁
+  let cmds ← prepareSmtQuery hs₂.toList (← mv₂.getType) fvNames₁
   let cmds := .setLogic "ALL" :: cmds
   if cfg.showQuery then
     logInfo m!"goal: {goalType}\n\nquery:\n{Command.cmdsAsQuery (cmds ++ [.checkSat])}"
     -- Return original goal.
-    return [mv]
+    return .unsat [mv] hs
   else
     trace[smt] "goal: {goalType}"
     trace[smt] "\nquery:\n{Command.cmdsAsQuery (cmds ++ [.checkSat])}"
@@ -118,28 +88,57 @@ def smt (cfg : Config) (mv : MVarId) (hs : Auto.InputHints') : MetaM (List MVarI
   match res with
   | .error e =>
     -- 5a. Print error reason.
-    trace[smt] "\nerror reason:\n{repr e}\n"
-    throwError "unable to prove goal, either it is false or you need to define more symbols with `smt [foo, bar]`"
-  | .ok pf =>
-    if cfg.trust then
-      -- 5b. Trust the result by admitting original goal.
-      mv.admit true
-      return []
-    -- 5c. Reconstruct proof.
+    trace[smt.solve] "\nerror:\n{repr e}\n"
+    throwError e.toString
+  | .ok (.unknown r) =>
+    -- 5b. Print unknown reason.
+    trace[smt.solve] "\nunknown reason:\n{r}\n"
+    return .unknown r.toString
+  | .ok (.unsat pf uc) =>
+    -- 5.d Reconstruct unsat core proofs.
     let ctx := { userNames := fvNames₂, native := cfg.native }
+    let (uc, _) ← (uc.mapM Reconstruct.reconstructTerm).run ctx {}
+    trace[smt] "unsat core: {uc}"
+    let ts₂ ← hs₂.mapM Meta.inferType
+    let uc := uc.filterMap fun p => ts₂.findIdx? (· == p) >>= (hs₂[·]?)
+    let uc := uc.filterMap (map₂[·]?)
+    let uc := uc.flatten.filterMap (map₁[·]?)
+    let uc := hs.filter uc.flatten.contains
+    if cfg.trust then
+      -- 6. Trust the result by admitting original goal.
+      mv.admit true
+      return .unsat [] uc
+    -- 7. Reconstruct proof.
     let (_, ps, p, hp, mvs) ← reconstructProof pf ctx
     let mv₂ ← mv₂.assert (← mkFreshId) p hp
     let ⟨_, mv₂⟩ ← mv₂.intro1
     let mut gs ← mv₂.apply (← Meta.mkAppOptM ``Prop.implies_of_not_and #[listExpr ps.dropLast q(Prop), goalType])
     mv₂.withContext (gs.forM (·.assumption))
     mv.assign (.mvar mv₁)
-    return mvs
+    return .unsat mvs uc
+  | .ok (.sat model) =>
+    -- 5e. Return potential counter-example.
+    if !cfg.model then
+      return .sat none
+    let (uss, es) := model.iss.unzip
+    let cs := es.map Array.size
+    let sortCard := Std.HashMap.insertMany ∅ (uss.zip cs)
+    let ctx := { userNames := fvNames₂, sortCard := sortCard, native := cfg.native }
+    let (uss', _) ← (uss.mapM Reconstruct.reconstructSort).run ctx {}
+    let cs' := cs.map (fun n => .app (.const ``Fin []) (@toExpr Nat Lean.instToExprNat n))
+    let state := { sortCache := Std.HashMap.insertMany ∅ (uss.zip cs') }
+    let (ufs, vs) := model.ifs.unzip
+    let (ufs', state) ← (ufs.mapM Reconstruct.reconstructTerm).run ctx state
+    let (vs', _) ← (vs.mapM Reconstruct.reconstructTerm).run ctx state
+    return .sat (.some (uss'.zip cs' ++ ufs'.zip vs'))
 
 namespace Tactic
 
 syntax smtStar := "*"
 
-syntax smtHints := (" [" withoutPosition((smtStar <|> term),*,?) "]")?
+syntax smtHintElem := smtStar <|> term
+
+syntax smtHints := (" [" withoutPosition(smtHintElem,*,?) "]")?
 
 open Lean.Parser.Tactic in
 /-- `smt` converts the current goal into an SMT query and checks if it is
@@ -187,6 +186,18 @@ Please take a look at the `Smt.Config` structure for more options.
 syntax (name := smt) "smt " optConfig smtHints : tactic
 
 open Lean.Parser.Tactic in
+/--
+`smt?` takes the same arguments as `smt`, but reports an equivalent call to
+`smt` that would be sufficient to close the goal. This is useful for reducing
+the size of the hints in a local invocation to speed up processing.
+```
+example (x : Nat) : (if True then x + 2 else 3) = x + 2 := by
+  smt? -- prints "Try this: simp only [ite_true]"
+```
+-/
+syntax (name := smtTrace) "smt?" optConfig smtHints : tactic
+
+open Lean.Parser.Tactic in
 /-- `smt_show` is short-hand for `smt +showQuery`. -/
 macro "smt_show " c:optConfig h:smtHints : tactic => do
   let `(optConfig| $cs*) := c | Macro.throwUnsupported
@@ -197,18 +208,69 @@ macro "smt_show " c:optConfig h:smtHints : tactic => do
 
 declare_config_elab elabConfig Smt.Config
 
-def elabHints : TSyntax `smtHints → TacticM (Auto.InputHints')
-  | `(smtHints| [ $[$hs],* ]) => withMainContext do
-    hs.foldrM (init := ⟨#[], #[], false⟩) fun h acc => do
-      if h.getKind == ``Smt.Tactic.smtStar then
-        return { acc with lctxhyps := true }
-      let h ← Auto.Prep.elabLemma ⟨h⟩ (.leaf s!"❰{h}❱")
-      return { acc with lemmas := acc.lemmas.push h }
-  | `(smtHints| ) => return ⟨#[], #[], false⟩
+def elabSmtHintElem : TSyntax ``smtHintElem → TacticM (Array (Expr × (TSyntax ``smtHintElem)) × Array Expr)
+  | `(smtHintElem| *) => do
+    let fvs ← Smt.Preprocess.getPropHyps
+    let hs := fvs.map Expr.fvar
+    let lctx ← getLCtx
+    let ss : Array (TSyntax ``smtHintElem) ← fvs.mapM fun fv => do
+      if let some ldecl := lctx.find? fv then
+        if !ldecl.userName.isInaccessibleUserName && !ldecl.userName.hasMacroScopes &&
+            (lctx.findFromUserName? ldecl.userName).get!.fvarId == ldecl.fvarId then
+          `(smtHintElem| $(mkIdent ldecl.userName):ident)
+        else
+          `(smtHintElem| *)
+      else
+        `(smtHintElem| *)
+    return (hs.zip ss, hs)
+  | `(smtHintElem| $h:term) => do
+    let h' ← Auto.Prep.elabLemma h (.leaf s!"❰{h}❱")
+    return (#[(h'.proof, ← `(smtHintElem| $h:term))], #[h'.proof])
   | _ => throwUnsupportedSyntax
 
-@[tactic smt] def evalSmt : Tactic := fun stx => withMainContext do
-  let mvs ← Smt.smt (← elabConfig stx[1]) (← Tactic.getMainGoal) (← elabHints ⟨stx[2]⟩)
-  Tactic.replaceMainGoal mvs
+def elabHints : TSyntax ``smtHints → TacticM (Std.HashMap Expr (TSyntax ``smtHintElem) × Array Expr)
+  | `(smtHints| [ $[$hs],* ]) => withMainContext do
+    hs.foldlM (init := ({}, #[])) fun (map, acc) h => do
+      let (m, a) ← elabSmtHintElem h
+      return (map.insertMany m, acc ++ a)
+  | `(smtHints| ) => return ({}, #[])
+  | _ => throwUnsupportedSyntax
+
+def evalSmtCore (cfg : TSyntax ``Parser.Tactic.optConfig) (hs : TSyntax ``smtHints) := withMainContext do
+  let cfg ← elabConfig cfg
+  let mv ← Tactic.getMainGoal
+  let (map, hs) ← elabHints hs
+  let res ← Smt.smt cfg mv hs
+  match res with
+    | .sat none =>
+      throwError "unable to prove goal, either it is false or you need to define more symbols. Try adding '+model' config option to display a potential counter-example (experimental)."
+    | .sat (.some model) =>
+      if model.isEmpty then
+        throwError "unable to prove goal, either it is false or you need to define more symbols. Could not produce a counter-example. Try introducing variables into the local context to get a counter-example."
+      else
+        let mut md := m!""
+        for (v, t) in model do
+          md := md ++ m!"\n  {v} = {t}"
+        throwError "unable to prove goal, either it is false or you need to define more symbols. Here is a potential counter-example:\n{md}"
+    | .unsat mvs uc =>
+      Tactic.replaceMainGoal mvs
+      let uc := uc.filterMap map.get?
+      let uc := uc.toList.eraseDups.toArray
+      return uc
+    | .unknown r =>
+      throwError "unable to prove goal. Try providing more hints. Reason: {r}"
+
+@[tactic smt] def evalSmt : Tactic := fun stx => match stx with
+  | `(tactic| smt $cfg:optConfig $hs:smtHints) => do
+    _ ← evalSmtCore cfg hs
+  | _ => throwUnsupportedSyntax
+
+@[tactic smtTrace] def evalSmtTrace : Tactic := fun stx => withMainContext do
+  match stx with
+  | `(tactic| smt?%$tk $cfg:optConfig $hs:smtHints) => do
+    let uc ← evalSmtCore cfg hs
+    let stx ← if uc.isEmpty then `(tactic| smt%$tk) else `(tactic| smt%$tk $cfg [$uc,*])
+    Lean.Meta.Tactic.TryThis.addSuggestion tk stx (origSpan? := ← getRef)
+  | _ => throwUnsupportedSyntax
 
 end Smt.Tactic
