Smt/Preprocess/PushHintsToCtx.lean
@@ -1,0 +1,27 @@
+/-
+Copyright (c) 2021-2024 by the authors listed in the file AUTHORS and their
+institutional affiliations. All rights reserved.
+Released under Apache 2.0 license as described in the file LICENSE.
+Authors: Abdalrhman Mohamed
+-/
+
+import Smt.Preprocess.Basic
+import Lean.Meta.Tactic.Assert
+
+namespace Smt.Preprocess
+
+open Lean
+
+def pushHintsToCtx (mv : MVarId) (hs : Array Expr) : MetaM Result := do
+  hs.foldrM pushHint { map := {}, hs := #[], mv }
+where
+  pushHint (h : Expr) (r : Result) : MetaM Result := do
+    if h.isFVar || h.isConst then
+      return { r with map := r.map.insert h #[h], hs := r.hs.push h }
+    else
+      let mv' ← r.mv.assert (← mkFreshId) (← Meta.inferType h) h
+      let ⟨fv, mv'⟩ ← mv'.intro1
+      let h' := .fvar fv
+      return { map := r.map.insert h' #[h], hs := r.hs.push h', mv := mv' }
+
+end Smt.Preprocess
